upd

Run.v
@@ -1,7 +1,7 @@
-Require Import Relations Arith Turing Alphabet Bool.
+Require Import List Relations Arith Turing Alphabet Bool.
 
 Section Run.
-  Variable state: Type.
+  Context {state: Type}.
   Variable initial: state.
   Variable step_rel: relation state.
 
@@ -19,36 +19,130 @@ Section Run.
 End Run.
 
 Section RunTuring.
-  Variable state_count symbol_count: positive.
+  Context {state_count symbol_count: positive}.
 
-  Local Definition machine := machine state_count symbol_count.
+  Local Definition machine := turing_machine state_count symbol_count.
   Local Definition state := alphabet state_count.
   Local Definition symbol := alphabet symbol_count.
-  Local Definition tape := tape symbol_count.
+  Local Definition tape := str symbol_count.
   Local Definition State: Set := state * tape * tape.
-  Local Definition head := head symbol_count.
-  Local Definition tail := tail symbol_count.
-  Local Definition blank_sym := blank symbol_count.
-  Local Definition blank_state := blank state_count.
+  Local Definition blank := sym_0 symbol_count.
+  Local Definition initial := sym_0 state_count.
 
   Variable m: machine.
-  Variable initial: state = sym_0 state_count.
   Variable program input: tape.
   Local Definition Initial: State := (initial, program, input).
-  Local Definition m_step := step state_count symbol_count m.
-  Local Definition m_steps := steps State m_step.
+  Local Definition m_step := step m.
+  Local Definition m_steps := steps m_step.
 
-  Definition tm_halts := halts State Initial m_step.
-  Definition tm_halted (s: State) := halted State s m_step.
+  Local Definition tm_halts := halts Initial m_step.
+  Local Definition tm_halted (s: State) := halted s m_step.
 
-  Local Definition m_runtime_func := runtime_func State Initial m_step.
+  Local Definition m_runtime_func := runtime_func Initial m_step.
 
-  Local Definition next_steps' (s: State) (i: state) (j: symbol): list State :=
-  nil.
+  Local Definition next_steps_point (s: State) (i: state) (j: symbol): list State :=
+    let (st'l, r) := s in let (st, l) := st'l in
+    match m st (head r) i j Left with
+    | false => nil
+    | true => cons (go_left (i, l, r) j) nil
+    end ++
+    match m st (head r) i j Right with
+    | false => nil
+    | true => cons (go_right (i, l, r) j) nil
+    end.
 
-  Definition next_steps (s: State): list State := next_steps' s blank_state blank_sym.
+  Local Lemma next_steps_point_correct:
+    forall (s s': State),
+    let (st'l, r) := s' in let (st, l) := st'l in
+    m_step s s' -> In s' (next_steps_point s st (head (tail r))) \/
+                   In s' (next_steps_point s st (head l)).
+  Proof.
+    destruct s as [st'l r].
+    destruct st'l as [st l].
+    destruct s' as [st'l' r'].
+    destruct st'l' as [st' l'].
+    intros.
+    unfold next_steps_point.
+    inversion H; subst.
+    assert (head (head r :: sym' :: tail r) = head r). unfold head. unfold hd. auto.
+    destruct d.
+    - left.
+      unfold go_d in H5.
+      remember H5 as H7. clear HeqH7.
+      apply go_left_state in H7.
+      apply go_left_sym in H5.
+      rewrite <- H5.
+      rewrite <- H7.
+      rewrite H2. simpl. auto.
+    - right.
+      unfold go_d in H5.
+      remember H5 as H7. clear HeqH7.
+      apply go_right_state in H7.
+      apply go_right_sym in H5.
+      rewrite <- H5.
+      rewrite <- H7.
+      rewrite H2. simpl.
+      intuition.
+  Qed.
 
-  Definition is_halted (s: State) := next_steps s = nil.
+  Local Fixpoint next_steps' (s: State) (i: state) (j: symbol) (k: nat): list State.
+    remember (next_steps_point s i j) as rest.
+    destruct k. exact rest.
+
+    destruct i as [n_i prf_i].
+    destruct (sym_dec state_count (S n_i)) as [prf_i'|prf_i'].
+    - remember (nat_to_sym state_count (S n_i) prf_i') as i'.
+      exact (rest ++ (next_steps' s i' j (k-1))).
+    - destruct j as [n_j prf_j].
+      destruct (sym_dec symbol_count (S n_j)) as [prf_j'|prf_j'].
+      + remember (nat_to_sym symbol_count (S n_j) prf_j') as j'.
+        exact (rest ++ (next_steps' s initial j' (k-1))).
+      + exact rest.
+  Defined.
+
+  Definition next_steps (s: State): list State :=
+    next_steps' s initial blank (state_count * symbol_count).
+
+  Theorem next_steps_correct: forall (s s': State), m_step s s' <-> In s' (next_steps s).
+  Proof.
+
+  Admitted.
+
+  Definition is_halted (s: State) :=
+    match next_steps s with
+    | nil => true
+    | _ => false
+    end.
+
+  Theorem is_halted_correct: forall (s: State), tm_halted s <-> is_halted s = true.
+  Proof.
+    intros.
+    unfold is_halted.
+    unfold tm_halted.
+    unfold halted.
+    split; intros.
+    - destruct (next_steps s) eqn:Hs; auto.
+      remember (List.in_eq s0 l) as Hin.
+      clear HeqHin.
+      rewrite <- Hs in Hin.
+      apply <- next_steps_correct in Hin.
+      exfalso.
+      exact (H s0 Hin).
+    - intro.
+      destruct (next_steps s) eqn:Hs.
+      + apply next_steps_correct in H0.
+        rewrite Hs in H0.
+        exact (List.in_nil H0).
+      + inversion H.
+  Qed.
+
+
+  Definition read_decision (s: State) :=
+    let (st'l, r) := s in
+    match sym_to_nat (head r) with
+    | 0 => false
+    | _ => true
+    end.
 
   Inductive decision: bool -> Prop :=
   | Rejects: tm_halts -> (
@@ -60,7 +154,11 @@ Section RunTuring.
         tm_halted (s, l, r) /\ m_steps Initial (s, l, r) /\ sym_to_nat (head r) <> 0
     ) -> decision true.
 
-  Fixpoint simulate (s: State) (n: nat).
+
+
+  Fixpoint simulate (n: nat) (s: State): option bool :=
+    if is_halted s then read_decision s
+    else 
 
   Theroem simulate_implies_halt: .
   Proof.
@@ -72,3 +170,9 @@ Section RunTuring.
 
   Qed.
 End RunTuring.
+
+Section Decision'.
+  Definition decision': .
+  language_of
+
+End Decision'.
