Language.v
@@ -2,6 +2,6 @@ Require Import Arith List Alphabet.
 
 Section Language.
   Local Lemma two_gte_one: 2 >= 1. Proof. auto. Qed.
-  Definition binstr := list (alphabet (nat_to_atl 1 2 two_gte_one)).
+  Definition binstr := str (nat_to_atl 1 2 two_gte_one).
   Definition language := binstr -> Prop.
 End Language.
